<h1>Equation Simplification</h1>

I started with the given equation which was F=A'B'C'+A'B'C+A'BC+AB'C+ABC'

I factored out the A'B' from the first two terms. 
Then I had F=A'B'(C'+C)+A'BC+AB'C+ABC'

I know that because of Complement (OR) the C' + C can be simplified to a 1. 
And this would make the equation F=A'B'+A'BC+AB'C+ABC'

Then, I can factor the B' out of the first two terms.
This gives me F=B'(A'+AC)+AB'C+ABC'
I can use the absorption law inside the parenthesis to simplify the A'+AC to A' + C
So now I have F=B'(A'+C)+AB'C+ABC'
